an allocation lemma

theories/semtype.v
@@ -2,6 +2,7 @@ From stdpp Require Import base.
 From iris.base_logic Require Import upred.
 From iris.base_logic.lib Require Import iprop own.
 From iris.algebra Require Import ofe cmra gmap_view.
+From iris.proofmode Require Import tactics.
 
 Definition tag := positive.
 Definition loc := positive.
@@ -9,17 +10,19 @@ Inductive value : Set :=
   | UnitV
   | LocV (ℓ : loc).
 
+Local Instance value_inhabited : Inhabited value := populate UnitV.
+
 Canonical Structure tagO : ofe := discreteO tag.
 
 (* interpretation of types *)
 Definition sem_typeO (Σ : gFunctors) : ofe := value -d> iPropO Σ.
 
 Class sem_heapG (Σ : gFunctors) : Set := SemHeapG {
-  sem_heapG_inv :> inG Σ (gmap_viewR loc (prodO tagO (laterO (sem_typeO Σ))))
+  sem_heapG_heap :> inG Σ (gmap_viewR loc (prodO tagO (laterO (sem_typeO Σ))));
 }.
 
 Section proofs.
-Context `{sem_heapG Σ}.
+Context `{!sem_heapG Σ}.
 Notation iProp := (iProp Σ).
 
 Inductive langty := 
@@ -40,29 +43,66 @@ Definition interp_unit : interp :=
 Definition interp_union (iA : interp) (iB : interp) : interp :=
   λ (w : value), (iA w ∨ iB w)%I.
 
+(* name for the semantic heap *)
+Context (γ : gname).
+
+Notation sem_heap_mapsto ℓ t iF :=
+  (own γ (gmap_view_frag ℓ DfracDiscarded (t, Next iF))).
+
 (* interpret a class type given the tag and the
    interpretation for the unique field type *)
-Definition interp_class (γ : gname) (t : tag) (iF : interp) : interp :=
-  λ (w : value), (
-    ∃ ℓ, ⌜w = LocV ℓ⌝ ∗ own γ (gmap_view_frag ℓ DfracDiscarded (t, Next iF))
-  )%I.
+Definition interp_class (t : tag) (iF : interp) : interp :=
+  λ (w : value), (∃ ℓ, ⌜w = LocV ℓ⌝ ∗ sem_heap_mapsto ℓ t iF)%I.
 
-From iris.proofmode Require Import tactics.
-
-(* sanity check that the own assertion is persistent *)
-Lemma frag_test (γ : gname) (ℓ : loc) x :
-  own γ (gmap_view_frag ℓ DfracDiscarded x) -∗
-  own γ (gmap_view_frag ℓ DfracDiscarded x) ∗
-  own γ (gmap_view_frag ℓ DfracDiscarded x).
-Proof.
-  iStartProof. iIntros "#Hown". by iSplitL.
-Qed.
-
-Fixpoint interp_type (γ : gname) (ty : langty) : interp :=
+Fixpoint interp_type (ty : langty) : interp :=
   match ty with
   | UnitT => interp_unit
-  | UnionT A B => interp_union (interp_type γ A) (interp_type γ B)
-  | ClassT t F => interp_class γ t (interp_type γ F)
+  | UnionT A B => interp_union (interp_type A) (interp_type B)
+  | ClassT t F => interp_class t (interp_type F)
   end.
+
+(* concrete heaps *)
+Definition heap : Type := gmap loc (tag * value).
+
+(* heap models relation; the semantic heap does
+   not appear because it is hidden in iProp  *)
+Definition heap_models (h : heap) : iProp :=
+  ∃ sh,
+    own γ (gmap_view_auth 1 sh) ∗ ⌜dom (gset loc) sh = dom _ h⌝ ∗
+    ∀ (ℓ : loc) (t : tag) (v : value),
+      ⌜h !! ℓ = Some (t, v)⌝ -∗
+        ∃ (iF : interp), ⌜sh !! ℓ = Some (t, Next iF)⌝ ∗ iF v.
+
+(* the tag for a class C with a single unit field *)
+Definition tC : tag := 1%positive.
+
+Lemma alloc_unit_class_lemma (h : heap) (new : loc) :
+  h !! new = None →
+  heap_models h -∗ |==>
+   heap_models (<[ new := (tC, UnitV) ]> h) ∗
+   sem_heap_mapsto new tC (interp_type UnitT).
+Proof.
+  move=> Hnew. iIntros "Hm". iDestruct "Hm" as (sh) "[Hown [Hdom Hm]]".
+  iDestruct "Hdom" as %Hdom.
+  iMod (own_update with "Hown") as "[Hown Hfrag]".
+  { apply (gmap_view_alloc _ new DfracDiscarded); last done.
+    (* the typeclasses seem to be messed up below, I should be able
+       to use not_elem_of_dom directly *) 
+    move: Hnew. rewrite -!(@not_elem_of_dom _ _ (gset loc)).
+    by move: Hdom => ->. }
+  iIntros "!>". iFrame.
+  iExists _. iFrame. iSplitR.
+  { iPureIntro. rewrite !dom_insert_L.
+    by move: Hdom => ->. }
+  iIntros (ℓ t v) "Hlook".
+  rewrite lookup_insert_Some.
+  iDestruct "Hlook" as %[[<- [= <- <-]]|[Hℓ Hlook]].
+  - iExists _. rewrite lookup_insert.
+    iSplitR; first done.
+    by rewrite /= /interp_unit.
+  - iDestruct ("Hm" with "[]") as (iF) "[% HiF]"; first done.
+    iExists _. rewrite lookup_insert_ne; last done.
+    by iSplitR.
+Qed.
 
 End proofs.
